examples/sf/Smallstep.v
@@ -1,0 +1,1234 @@
+(* QuickChick Prelude *)
+Set Warnings "-extraction-opaque-accessed,-extraction".
+Set Warnings "-notation-overridden,-parsing".
+
+Require Import String List. Open Scope string.
+
+From QuickChick Require Import QuickChick Tactics.
+From mathcomp Require Import ssreflect ssrfun ssrbool ssrnat eqtype seq.
+Import QcDefaultNotation. Open Scope qc_scope.
+
+Set Bullet Behavior "Strict Subproofs".
+
+Require Import ZoeStuff.
+(* End prelude *)
+
+(** * Smallstep: Small-step Operational Semantics *)
+
+Require Import Coq.Arith.Arith.
+Require Import Coq.Arith.EqNat.
+Require Import Coq.omega.Omega.
+Require Import Coq.Lists.List.
+Import ListNotations.
+Require Import Maps.
+Require Import Imp.
+
+Inductive tm : Type :=
+  | C : nat -> tm         (* Constant *)
+  | P : tm -> tm -> tm.   (* Plus *)
+
+Fixpoint evalF (t : tm) : nat :=
+  match t with
+  | C n => n
+  | P a1 a2 => evalF a1 + evalF a2
+  end.
+
+
+Reserved Notation " t '\\' n " (at level 50, left associativity).
+
+Inductive eval : tm -> nat -> Prop :=
+  | E_Const : forall n,
+      C n \\ n
+  | E_Plus : forall t1 t2 n1 n2,
+      t1 \\ n1 ->
+      t2 \\ n2 ->
+      P t1 t2 \\ (n1 + n2)
+
+  where " t '\\' n " := (eval t n).
+
+Module SimpleArith1.
+
+Reserved Notation " t '===>' t' " (at level 55).
+
+Inductive step : tm -> tm -> Prop :=
+  | ST_PlusConstConst : forall n1 n2,
+      P (C n1) (C n2) ===> C (n1 + n2)
+  | ST_Plus1 : forall t1 t1' t2,
+      t1 ===> t1' ->
+      P t1 t2 ===> P t1' t2
+  | ST_Plus2 : forall n1 t2 t2',
+      t2 ===> t2' ->
+      P (C n1) t2 ===> P (C n1) t2'
+
+  where " t '===>' t' " := (step t t').
+
+End SimpleArith1.
+
+Definition relation (X: Type) := X->X->Prop.
+
+Definition deterministic {X: Type} (R: relation X) :=
+  forall x y1 y2 : X, R x y1 -> R x y2 -> y1 = y2.
+
+Module SimpleArith2.
+Import SimpleArith1.
+
+Theorem step_deterministic:
+  deterministic step.
+Admitted. (* Higher order *) 
+
+End SimpleArith2.
+
+Ltac solve_by_inverts n :=
+  match goal with | H : ?T |- _ => 
+  match type of T with Prop =>
+    solve [ 
+      inversion H; 
+      match n with S (S (?n')) => subst; solve_by_inverts (S n') end ]
+  end end.
+
+Ltac solve_by_invert :=
+  solve_by_inverts 1.
+
+
+Module SimpleArith3.
+Import SimpleArith1.
+
+Theorem step_deterministic_alt: deterministic step.
+Admitted. 
+
+End SimpleArith3.
+
+Inductive value : tm -> Prop :=
+  | v_const : forall n, value (C n).
+
+Derive ArbitrarySizedSuchThat for (fun t => value t).
+
+Reserved Notation " t '===>' t' " (at level 40).
+
+Inductive step : tm -> tm -> Prop :=
+  | ST_PlusConstConst : forall n1 n2,
+          P (C n1) (C n2)
+      ===> C (n1 + n2)
+  | ST_Plus1 : forall t1 t1' t2,
+        t1 ===> t1' ->
+        P t1 t2 ===> P t1' t2
+  | ST_Plus2 : forall v1 t2 t2',
+        value v1 ->                     (* <----- n.b. *)
+        t2 ===> t2' ->
+        P v1 t2 ===> P v1 t2'
+
+  where " t '===>' t' " := (step t t').
+
+Theorem step_deterministic :
+  deterministic step.
+Admitted. 
+
+Theorem strong_progress : forall t,
+  value t \/ (exists t', t ===> t').
+Admitted. (* Existential *)
+
+Definition normal_form {X:Type} (R:relation X) (t:X) : Prop :=
+  ~ exists t', R t t'.
+
+Lemma value_is_nf : forall v,
+  value v -> normal_form step v.
+Admitted. (* Existential *)
+
+Lemma nf_is_value : forall t,
+  normal_form step t -> value t.
+Admitted. (* Existential *)
+
+
+Module Temp1.
+
+Inductive value : tm -> Prop :=
+| v_const : forall n, value (C n)
+| v_funny : forall t1 n2,                       (* <---- *)
+              value (P t1 (C n2)).
+
+Reserved Notation " t '===>' t' " (at level 40).
+
+Inductive step : tm -> tm -> Prop :=
+  | ST_PlusConstConst : forall n1 n2,
+      P (C n1) (C n2) ===> C (n1 + n2)
+  | ST_Plus1 : forall t1 t1' t2,
+      t1 ===> t1' ->
+      P t1 t2 ===> P t1' t2
+  | ST_Plus2 : forall v1 t2 t2',
+      value v1 ->
+      t2 ===> t2' ->
+      P v1 t2 ===> P v1 t2'
+
+  where " t '===>' t' " := (step t t').
+
+Lemma value_not_same_as_normal_form :
+  exists v, value v /\ ~ normal_form step v.
+Proof.
+  (* FILL IN HERE *) Admitted.
+End Temp1.
+
+(** [] *)
+
+(** **** Exercise: 2 stars, optional (value_not_same_as_normal_form2)  *)
+(** Alternatively, we might mistakenly define [step] so that it
+    permits something designated as a value to reduce further. *)
+
+Module Temp2.
+
+Inductive value : tm -> Prop :=
+| v_const : forall n, value (C n).
+
+Reserved Notation " t '===>' t' " (at level 40).
+
+Inductive step : tm -> tm -> Prop :=
+  | ST_Funny : forall n,                         (* <---- *)
+      C n ===> P (C n) (C 0)
+  | ST_PlusConstConst : forall n1 n2,
+      P (C n1) (C n2) ===> C (n1 + n2)
+  | ST_Plus1 : forall t1 t1' t2,
+      t1 ===> t1' ->
+      P t1 t2 ===> P t1' t2
+  | ST_Plus2 : forall v1 t2 t2',
+      value v1 ->
+      t2 ===> t2' ->
+      P v1 t2 ===> P v1 t2'
+
+  where " t '===>' t' " := (step t t').
+
+Lemma value_not_same_as_normal_form :
+  exists v, value v /\ ~ normal_form step v.
+Proof.
+  (* FILL IN HERE *) Admitted.
+
+End Temp2.
+
+(** [] *)
+
+
+(** **** Exercise: 3 stars, optional (value_not_same_as_normal_form3)  *)
+(** Finally, we might define [value] and [step] so that there is some
+    term that is not a value but that cannot take a step in the [step]
+    relation.  Such terms are said to be _stuck_. In this case this is
+    caused by a mistake in the semantics, but we will also see
+    situations where, even in a correct language definition, it makes
+    sense to allow some terms to be stuck. *)
+
+Module Temp3.
+
+Inductive value : tm -> Prop :=
+  | v_const : forall n, value (C n).
+
+Reserved Notation " t '===>' t' " (at level 40).
+
+Inductive step : tm -> tm -> Prop :=
+  | ST_PlusConstConst : forall n1 n2,
+      P (C n1) (C n2) ===> C (n1 + n2)
+  | ST_Plus1 : forall t1 t1' t2,
+      t1 ===> t1' ->
+      P t1 t2 ===> P t1' t2
+
+  where " t '===>' t' " := (step t t').
+
+(** (Note that [ST_Plus2] is missing.) *)
+
+Lemma value_not_same_as_normal_form :
+  exists t, ~ value t /\ normal_form step t.
+Proof.
+  (* FILL IN HERE *) Admitted.
+
+End Temp3.
+
+
+(** [] *)
+
+(* ----------------------------------------------------------------- *)
+(** *** Additional Exercises *)
+
+Module Temp4.
+
+(** Here is another very simple language whose terms, instead of being
+    just addition expressions and numbers, are just the booleans true
+    and false and a conditional expression... *)
+
+Inductive tm : Type :=
+  | ttrue : tm
+  | tfalse : tm
+  | tif : tm -> tm -> tm -> tm.
+
+Inductive value : tm -> Prop :=
+  | v_true : value ttrue
+  | v_false : value tfalse.
+
+Reserved Notation " t '===>' t' " (at level 40).
+
+Inductive step : tm -> tm -> Prop :=
+  | ST_IfTrue : forall t1 t2,
+      tif ttrue t1 t2 ===> t1
+  | ST_IfFalse : forall t1 t2,
+      tif tfalse t1 t2 ===> t2
+  | ST_If : forall t1 t1' t2 t3,
+      t1 ===> t1' ->
+      tif t1 t2 t3 ===> tif t1' t2 t3
+
+  where " t '===>' t' " := (step t t').
+
+(** **** Exercise: 1 starM (smallstep_bools)  *)
+(** Which of the following propositions are provable?  (This is just a
+    thought exercise, but for an extra challenge feel free to prove
+    your answers in Coq.) *)
+
+Definition bool_step_prop1 :=
+  tfalse ===> tfalse.
+
+(* FILL IN HERE *)
+
+Definition bool_step_prop2 :=
+     tif
+       ttrue
+       (tif ttrue ttrue ttrue)
+       (tif tfalse tfalse tfalse)
+  ===>
+     ttrue.
+
+(* FILL IN HERE *)
+
+Definition bool_step_prop3 :=
+     tif
+       (tif ttrue ttrue ttrue)
+       (tif ttrue ttrue ttrue)
+       tfalse
+   ===>
+     tif
+       ttrue
+       (tif ttrue ttrue ttrue)
+       tfalse.
+
+(* FILL IN HERE *)
+(** [] *)
+
+(** **** Exercise: 3 stars, optional (progress_bool)  *)
+(** Just as we proved a progress theorem for plus expressions, we can
+    do so for boolean expressions, as well. *)
+
+Theorem strong_progress : forall t,
+  value t \/ (exists t', t ===> t').
+Proof.
+  (* FILL IN HERE *) Admitted.
+(** [] *)
+
+(** **** Exercise: 2 stars, optional (step_deterministic)  *)
+Theorem step_deterministic :
+  deterministic step.
+Proof.
+  (* FILL IN HERE *) Admitted.
+(** [] *)
+
+Module Temp5.
+
+(** **** Exercise: 2 stars (smallstep_bool_shortcut)  *)
+(** Suppose we want to add a "short circuit" to the step relation for
+    boolean expressions, so that it can recognize when the [then] and
+    [else] branches of a conditional are the same value (either
+    [ttrue] or [tfalse]) and reduce the whole conditional to this
+    value in a single step, even if the guard has not yet been reduced
+    to a value. For example, we would like this proposition to be
+    provable:
+
+         tif
+            (tif ttrue ttrue ttrue)
+            tfalse
+            tfalse
+     ===>
+         tfalse.
+*)
+
+(** Write an extra clause for the step relation that achieves this
+    effect and prove [bool_step_prop4]. *)
+
+Reserved Notation " t '===>' t' " (at level 40).
+
+Inductive step : tm -> tm -> Prop :=
+  | ST_IfTrue : forall t1 t2,
+      tif ttrue t1 t2 ===> t1
+  | ST_IfFalse : forall t1 t2,
+      tif tfalse t1 t2 ===> t2
+  | ST_If : forall t1 t1' t2 t3,
+      t1 ===> t1' ->
+      tif t1 t2 t3 ===> tif t1' t2 t3
+  (* FILL IN HERE *)
+
+  where " t '===>' t' " := (step t t').
+
+Definition bool_step_prop4 :=
+         tif
+            (tif ttrue ttrue ttrue)
+            tfalse
+            tfalse
+     ===>
+         tfalse.
+
+Example bool_step_prop4_holds :
+  bool_step_prop4.
+Proof.
+  (* FILL IN HERE *) Admitted.
+(** [] *)
+
+(** **** Exercise: 3 stars, optional (properties_of_altered_step)  *)
+(** It can be shown that the determinism and strong progress theorems
+    for the step relation in the lecture notes also hold for the
+    definition of step given above.  After we add the clause
+    [ST_ShortCircuit]...
+
+    - Is the [step] relation still deterministic?  Write yes or no and
+      briefly (1 sentence) explain your answer.
+
+      Optional: prove your answer correct in Coq. *)
+
+(* FILL IN HERE *)
+(**
+   - Does a strong progress theorem hold? Write yes or no and
+     briefly (1 sentence) explain your answer.
+
+     Optional: prove your answer correct in Coq.
+*)
+
+(* FILL IN HERE *)
+(**
+   - In general, is there any way we could cause strong progress to
+     fail if we took away one or more constructors from the original
+     step relation? Write yes or no and briefly (1 sentence) explain
+     your answer.
+
+(* FILL IN HERE *)
+*)
+(** [] *)
+
+End Temp5.
+End Temp4.
+
+(* ################################################################# *)
+(** * Multi-Step Reduction *)
+
+(** We've been working so far with the _single-step reduction_
+    relation [===>], which formalizes the individual steps of an
+    abstract machine for executing programs.
+
+    We can use the same machine to reduce programs to completion -- to
+    find out what final result they yield.  This can be formalized as
+    follows:
+
+    - First, we define a _multi-step reduction relation_ [===>*], which
+      relates terms [t] and [t'] if [t] can reach [t'] by any number
+      (including zero) of single reduction steps.
+
+    - Then we define a "result" of a term [t] as a normal form that
+      [t] can reach by multi-step reduction. *)
+
+
+(** Since we'll want to reuse the idea of multi-step reduction many
+    times, let's take a little extra trouble and define it
+    generically.
+
+    Given a relation [R], we define a relation [multi R], called the
+    _multi-step closure of [R]_ as follows. *)
+
+Inductive multi {X:Type} (R: relation X) : relation X :=
+  | multi_refl  : forall (x : X), multi R x x
+  | multi_step : forall (x y z : X),
+                    R x y ->
+                    multi R y z ->
+                    multi R x z.
+
+(** (In the [Rel] chapter and the Coq standard library, this relation
+    is called [clos_refl_trans_1n].  We give it a shorter name here
+    for the sake of readability.)
+
+    The effect of this definition is that [multi R] relates two
+    elements [x] and [y] if 
+
+       - [x = y], or 
+       - [R x y], or 
+       - there is some nonempty sequence [z1], [z2], ..., [zn] such that 
+
+           R x z1 
+           R z1 z2 
+           ...  
+           R zn y.
+
+    Thus, if [R] describes a single-step of computation, then [z1]...[zn] 
+    is the sequence of intermediate steps of computation between [x] and 
+    [y]. *)
+
+(** We write [===>*] for the [multi step] relation on terms. *)
+
+Notation " t '===>*' t' " := (multi step t t') (at level 40).
+
+(** The relation [multi R] has several crucial properties.
+
+    First, it is obviously _reflexive_ (that is, [forall x, multi R x
+    x]).  In the case of the [===>*] (i.e., [multi step]) relation, the
+    intuition is that a term can execute to itself by taking zero
+    steps of execution.
+
+    Second, it contains [R] -- that is, single-step executions are a
+    particular case of multi-step executions.  (It is this fact that
+    justifies the word "closure" in the term "multi-step closure of
+    [R].") *)
+
+Theorem multi_R : forall (X:Type) (R:relation X) (x y : X),
+       R x y -> (multi R) x y.
+Proof.
+  intros X R x y H.
+  apply multi_step with y. apply H. apply multi_refl.   Qed.
+
+(** Third, [multi R] is _transitive_. *)
+
+Theorem multi_trans :
+  forall (X:Type) (R: relation X) (x y z : X),
+      multi R x y  ->
+      multi R y z ->
+      multi R x z.
+Proof.
+  intros X R x y z G H.
+  induction G.
+    - (* multi_refl *) assumption.
+    - (* multi_step *)
+      apply multi_step with y. assumption.
+      apply IHG. assumption.  Qed.
+
+(** In particular, for the [multi step] relation on terms, if
+    [t1===>*t2] and [t2===>*t3], then [t1===>*t3]. *)
+
+(* ================================================================= *)
+(** ** Examples *)
+
+(** Here's a specific instance of the [multi step] relation: *)
+
+Lemma test_multistep_1:
+      P
+        (P (C 0) (C 3))
+        (P (C 2) (C 4))
+   ===>*
+      C ((0 + 3) + (2 + 4)).
+Proof.
+  apply multi_step with
+            (P (C (0 + 3))
+               (P (C 2) (C 4))).
+  apply ST_Plus1. apply ST_PlusConstConst.
+  apply multi_step with
+            (P (C (0 + 3))
+               (C (2 + 4))).
+  apply ST_Plus2. apply v_const.
+  apply ST_PlusConstConst.
+  apply multi_R.
+  apply ST_PlusConstConst. Qed.
+
+(** Here's an alternate proof of the same fact that uses [eapply] to
+    avoid explicitly constructing all the intermediate terms. *)
+
+Lemma test_multistep_1':
+      P
+        (P (C 0) (C 3))
+        (P (C 2) (C 4))
+  ===>*
+      C ((0 + 3) + (2 + 4)).
+Proof.
+  eapply multi_step. apply ST_Plus1. apply ST_PlusConstConst.
+  eapply multi_step. apply ST_Plus2. apply v_const.
+  apply ST_PlusConstConst.
+  eapply multi_step. apply ST_PlusConstConst.
+  apply multi_refl.  Qed.
+
+(** **** Exercise: 1 star, optional (test_multistep_2)  *)
+Lemma test_multistep_2:
+  C 3 ===>* C 3.
+Proof.
+  (* FILL IN HERE *) Admitted.
+(** [] *)
+
+(** **** Exercise: 1 star, optional (test_multistep_3)  *)
+Lemma test_multistep_3:
+      P (C 0) (C 3)
+   ===>*
+      P (C 0) (C 3).
+Proof.
+  (* FILL IN HERE *) Admitted.
+(** [] *)
+
+(** **** Exercise: 2 stars (test_multistep_4)  *)
+Lemma test_multistep_4:
+      P
+        (C 0)
+        (P
+          (C 2)
+          (P (C 0) (C 3)))
+  ===>*
+      P
+        (C 0)
+        (C (2 + (0 + 3))).
+Proof.
+  (* FILL IN HERE *) Admitted.
+(** [] *)
+
+(* ================================================================= *)
+(** ** Normal Forms Again *)
+
+(** If [t] reduces to [t'] in zero or more steps and [t'] is a
+    normal form, we say that "[t'] is a normal form of [t]." *)
+
+Definition step_normal_form := normal_form step.
+
+Definition normal_form_of (t t' : tm) :=
+  (t ===>* t' /\ step_normal_form t').
+
+(** We have already seen that, for our language, single-step reduction is
+    deterministic -- i.e., a given term can take a single step in
+    at most one way.  It follows from this that, if [t] can reach
+    a normal form, then this normal form is unique.  In other words, we
+    can actually pronounce [normal_form t t'] as "[t'] is _the_
+    normal form of [t]." *)
+
+(** **** Exercise: 3 stars, optional (normal_forms_unique)  *)
+Theorem normal_forms_unique:
+  deterministic normal_form_of.
+Proof.
+  (* We recommend using this initial setup as-is! *)
+  unfold deterministic. unfold normal_form_of.
+  intros x y1 y2 P1 P2.
+  inversion P1 as [P11 P12]; clear P1.
+  inversion P2 as [P21 P22]; clear P2.
+  generalize dependent y2.
+  (* FILL IN HERE *) Admitted.
+(** [] *)
+
+(** Indeed, something stronger is true for this language (though not
+    for all languages): the reduction of _any_ term [t] will
+    eventually reach a normal form -- i.e., [normal_form_of] is a
+    _total_ function.  Formally, we say the [step] relation is
+    _normalizing_. *)
+
+Definition normalizing {X:Type} (R:relation X) :=
+  forall t, exists t',
+    (multi R) t t' /\ normal_form R t'.
+
+(** To prove that [step] is normalizing, we need a couple of lemmas.
+
+    First, we observe that, if [t] reduces to [t'] in many steps, then
+    the same sequence of reduction steps within [t] is also possible
+    when [t] appears as the left-hand child of a [P] node, and
+    similarly when [t] appears as the right-hand child of a [P]
+    node whose left-hand child is a value. *)
+
+Lemma multistep_congr_1 : forall t1 t1' t2,
+     t1 ===>* t1' ->
+     P t1 t2 ===>* P t1' t2.
+Proof.
+  intros t1 t1' t2 H. induction H.
+    - (* multi_refl *) apply multi_refl.
+    - (* multi_step *) apply multi_step with (P y t2).
+        apply ST_Plus1. apply H.
+        apply IHmulti.  Qed.
+
+(** **** Exercise: 2 stars (multistep_congr_2)  *)
+Lemma multistep_congr_2 : forall t1 t2 t2',
+     value t1 ->
+     t2 ===>* t2' ->
+     P t1 t2 ===>* P t1 t2'.
+Proof.
+  (* FILL IN HERE *) Admitted.
+(** [] *)
+
+(** With these lemmas in hand, the main proof is a straightforward
+    induction.
+
+    _Theorem_: The [step] function is normalizing -- i.e., for every
+    [t] there exists some [t'] such that [t] steps to [t'] and [t'] is
+    a normal form.
+
+    _Proof sketch_: By induction on terms.  There are two cases to
+    consider:
+
+    - [t = C n] for some [n].  Here [t] doesn't take a step, and we
+      have [t' = t].  We can derive the left-hand side by reflexivity
+      and the right-hand side by observing (a) that values are normal
+      forms (by [nf_same_as_value]) and (b) that [t] is a value (by
+      [v_const]).
+
+    - [t = P t1 t2] for some [t1] and [t2].  By the IH, [t1] and [t2]
+      have normal forms [t1'] and [t2'].  Recall that normal forms are
+      values (by [nf_same_as_value]); we know that [t1' = C n1] and
+      [t2' = C n2], for some [n1] and [n2].  We can combine the [===>*]
+      derivations for [t1] and [t2] using [multi_congr_1] and
+      [multi_congr_2] to prove that [P t1 t2] reduces in many steps to
+      [C (n1 + n2)].
+
+      It is clear that our choice of [t' = C (n1 + n2)] is a value,
+      which is in turn a normal form. [] *)
+
+Theorem step_normalizing :
+  normalizing step.
+Admitted. 
+
+(* ================================================================= *)
+(** ** Equivalence of Big-Step and Small-Step *)
+
+(** Having defined the operational semantics of our tiny programming
+    language in two different ways (big-step and small-step), it makes
+    sense to ask whether these definitions actually define the same
+    thing!  They do, though it takes a little work to show it.  The
+    details are left as an exercise. *)
+
+(** **** Exercise: 3 stars (eval__multistep)  *)
+Theorem eval__multistep : forall t n,
+  t \\ n -> t ===>* C n.
+
+(** The key ideas in the proof can be seen in the following picture:
+
+       P t1 t2 ===>            (by ST_Plus1)
+       P t1' t2 ===>           (by ST_Plus1)
+       P t1'' t2 ===>          (by ST_Plus1)
+       ...
+       P (C n1) t2 ===>        (by ST_Plus2)
+       P (C n1) t2' ===>       (by ST_Plus2)
+       P (C n1) t2'' ===>      (by ST_Plus2)
+       ...
+       P (C n1) (C n2) ===>    (by ST_PlusConstConst)
+       C (n1 + n2)
+
+    That is, the multistep reduction of a term of the form [P t1 t2]
+    proceeds in three phases:
+       - First, we use [ST_Plus1] some number of times to reduce [t1]
+         to a normal form, which must (by [nf_same_as_value]) be a
+         term of the form [C n1] for some [n1].
+       - Next, we use [ST_Plus2] some number of times to reduce [t2]
+         to a normal form, which must again be a term of the form [C
+         n2] for some [n2].
+       - Finally, we use [ST_PlusConstConst] one time to reduce [P (C
+         n1) (C n2)] to [C (n1 + n2)]. *)
+
+(** To formalize this intuition, you'll need to use the congruence
+    lemmas from above (you might want to review them now, so that
+    you'll be able to recognize when they are useful), plus some basic
+    properties of [===>*]: that it is reflexive, transitive, and
+    includes [===>]. *)
+
+Proof.
+  (* FILL IN HERE *) Admitted.
+(** [] *)
+
+(** **** Exercise: 3 stars, advanced (eval__multistep_inf)  *)
+(** Write a detailed informal version of the proof of [eval__multistep].
+
+(* FILL IN HERE *)
+[]
+*)
+
+(** For the other direction, we need one lemma, which establishes a
+    relation between single-step reduction and big-step evaluation. *)
+
+(** **** Exercise: 3 stars (step__eval)  *)
+Lemma step__eval : forall t t' n,
+     t ===> t' ->
+     t' \\ n ->
+     t \\ n.
+Proof.
+  intros t t' n Hs. generalize dependent n.
+  (* FILL IN HERE *) Admitted.
+(** [] *)
+
+(** The fact that small-step reduction implies big-step evaluation is
+    now straightforward to prove, once it is stated correctly.
+
+    The proof proceeds by induction on the multi-step reduction
+    sequence that is buried in the hypothesis [normal_form_of t t']. *)
+
+(** Make sure you understand the statement before you start to
+    work on the proof.  *)
+
+(** **** Exercise: 3 stars (multistep__eval)  *)
+Theorem multistep__eval : forall t t',
+  normal_form_of t t' -> exists n, t' = C n /\ t \\ n.
+Proof.
+  (* FILL IN HERE *) Admitted.
+(** [] *)
+
+(* ================================================================= *)
+(** ** Additional Exercises *)
+
+(** **** Exercise: 3 stars, optional (interp_tm)  *)
+(** Remember that we also defined big-step evaluation of terms as a
+    function [evalF].  Prove that it is equivalent to the existing
+    semantics.  (Hint: we just proved that [eval] and [multistep] are
+    equivalent, so logically it doesn't matter which you choose.
+    One will be easier than the other, though!) *)
+
+Theorem evalF_eval : forall t n,
+  evalF t = n <-> t \\ n.
+Proof.
+  (* FILL IN HERE *) Admitted.
+(** [] *)
+
+(** **** Exercise: 4 starsM (combined_properties)  *)
+(** We've considered arithmetic and conditional expressions
+    separately.  This exercise explores how the two interact. *)
+
+Module Combined.
+
+Inductive tm : Type :=
+  | C : nat -> tm
+  | P : tm -> tm -> tm
+  | ttrue : tm
+  | tfalse : tm
+  | tif : tm -> tm -> tm -> tm.
+
+Inductive value : tm -> Prop :=
+  | v_const : forall n, value (C n)
+  | v_true : value ttrue
+  | v_false : value tfalse.
+
+Reserved Notation " t '===>' t' " (at level 40).
+
+Inductive step : tm -> tm -> Prop :=
+  | ST_PlusConstConst : forall n1 n2,
+      P (C n1) (C n2) ===> C (n1 + n2)
+  | ST_Plus1 : forall t1 t1' t2,
+      t1 ===> t1' ->
+      P t1 t2 ===> P t1' t2
+  | ST_Plus2 : forall v1 t2 t2',
+      value v1 ->
+      t2 ===> t2' ->
+      P v1 t2 ===> P v1 t2'
+  | ST_IfTrue : forall t1 t2,
+      tif ttrue t1 t2 ===> t1
+  | ST_IfFalse : forall t1 t2,
+      tif tfalse t1 t2 ===> t2
+  | ST_If : forall t1 t1' t2 t3,
+      t1 ===> t1' ->
+      tif t1 t2 t3 ===> tif t1' t2 t3
+
+  where " t '===>' t' " := (step t t').
+
+(** Earlier, we separately proved for both plus- and if-expressions...
+
+    - that the step relation was deterministic, and
+
+    - a strong progress lemma, stating that every term is either a
+      value or can take a step.
+
+    Prove or disprove these two properties for the combined language. *)
+
+(* FILL IN HERE *)
+
+End Combined.
+(** [] *)
+
+
+(* ################################################################# *)
+(** * Small-Step Imp *)
+
+(** Now for a more serious example: a small-step version of the Imp
+    operational semantics. *)
+
+(** The small-step reduction relations for arithmetic and
+    boolean expressions are straightforward extensions of the tiny
+    language we've been working up to now.  To make them easier to
+    read, we introduce the symbolic notations [===>a] and [===>b] for
+    the arithmetic and boolean step relations. *)
+
+Inductive aval : aexp -> Prop :=
+  | av_num : forall n, aval (ANum n).
+
+(** We are not actually going to bother to define boolean
+    values, since they aren't needed in the definition of [===>b]
+    below (why?), though they might be if our language were a bit
+    larger (why?). *)
+
+(*
+Reserved Notation " t '/' st '===>a' t' "
+                  (at level 40, st at level 39).
+
+Inductive astep : state -> aexp -> aexp -> Prop :=
+  | AS_Id : forall st i,
+      AId i / st ===>a ANum (st i)
+  | AS_Plus : forall st n1 n2,
+      APlus (ANum n1) (ANum n2) / st ===>a ANum (n1 + n2)
+  | AS_Plus1 : forall st a1 a1' a2,
+      a1 / st ===>a a1' ->
+      (APlus a1 a2) / st ===>a (APlus a1' a2)
+  | AS_Plus2 : forall st v1 a2 a2',
+      aval v1 ->
+      a2 / st ===>a a2' ->
+      (APlus v1 a2) / st ===>a (APlus v1 a2')
+  | AS_Minus : forall st n1 n2,
+      (AMinus (ANum n1) (ANum n2)) / st ===>a (ANum (minus n1 n2))
+  | AS_Minus1 : forall st a1 a1' a2,
+      a1 / st ===>a a1' ->
+      (AMinus a1 a2) / st ===>a (AMinus a1' a2)
+  | AS_Minus2 : forall st v1 a2 a2',
+      aval v1 ->
+      a2 / st ===>a a2' ->
+      (AMinus v1 a2) / st ===>a (AMinus v1 a2')
+  | AS_Mult : forall st n1 n2,
+      (AMult (ANum n1) (ANum n2)) / st ===>a (ANum (mult n1 n2))
+  | AS_Mult1 : forall st a1 a1' a2,
+      a1 / st ===>a a1' ->
+      (AMult a1 a2) / st ===>a (AMult a1' a2)
+  | AS_Mult2 : forall st v1 a2 a2',
+      aval v1 ->
+      a2 / st ===>a a2' ->
+      (AMult v1 a2) / st ===>a (AMult v1 a2')
+
+    where " t '/' st '===>a' t' " := (astep st t t').
+
+Reserved Notation " t '/' st '===>b' t' "
+                  (at level 40, st at level 39).
+
+Inductive bstep : state -> bexp -> bexp -> Prop :=
+| BS_Eq : forall st n1 n2,
+    (BEq (ANum n1) (ANum n2)) / st ===>b
+    (if (beq_nat n1 n2) then BTrue else BFalse)
+| BS_Eq1 : forall st a1 a1' a2,
+    a1 / st ===>a a1' ->
+    (BEq a1 a2) / st ===>b (BEq a1' a2)
+| BS_Eq2 : forall st v1 a2 a2',
+    aval v1 ->
+    a2 / st ===>a a2' ->
+    (BEq v1 a2) / st ===>b (BEq v1 a2')
+| BS_LtEq : forall st n1 n2,
+    (BLe (ANum n1) (ANum n2)) / st ===>b
+             (if (leb n1 n2) then BTrue else BFalse)
+| BS_LtEq1 : forall st a1 a1' a2,
+    a1 / st ===>a a1' ->
+    (BLe a1 a2) / st ===>b (BLe a1' a2)
+| BS_LtEq2 : forall st v1 a2 a2',
+    aval v1 ->
+    a2 / st ===>a a2' ->
+    (BLe v1 a2) / st ===>b (BLe v1 a2')
+| BS_NotTrue : forall st,
+    (BNot BTrue) / st ===>b BFalse
+| BS_NotFalse : forall st,
+    (BNot BFalse) / st ===>b BTrue
+| BS_NotStep : forall st b1 b1',
+    b1 / st ===>b b1' ->
+    (BNot b1) / st ===>b (BNot b1')
+| BS_AndTrueTrue : forall st,
+    (BAnd BTrue BTrue) / st ===>b BTrue
+| BS_AndTrueFalse : forall st,
+    (BAnd BTrue BFalse) / st ===>b BFalse
+| BS_AndFalse : forall st b2,
+    (BAnd BFalse b2) / st ===>b BFalse
+| BS_AndTrueStep : forall st b2 b2',
+    b2 / st ===>b b2' ->
+    (BAnd BTrue b2) / st ===>b (BAnd BTrue b2')
+| BS_AndStep : forall st b1 b1' b2,
+    b1 / st ===>b b1' ->
+    (BAnd b1 b2) / st ===>b (BAnd b1' b2)
+
+where " t '/' st '===>b' t' " := (bstep st t t').
+
+(** The semantics of commands is the interesting part.  We need two
+    small tricks to make it work:
+
+       - We use [SKIP] as a "command value" -- i.e., a command that
+         has reached a normal form.
+
+            - An assignment command reduces to [SKIP] (and an updated
+              state).
+
+            - The sequencing command waits until its left-hand
+              subcommand has reduced to [SKIP], then throws it away so
+              that reduction can continue with the right-hand
+              subcommand.
+
+       - We reduce a [WHILE] command by transforming it into a
+         conditional followed by the same [WHILE]. *)
+
+(** (There are other ways of achieving the effect of the latter
+    trick, but they all share the feature that the original [WHILE]
+    command needs to be saved somewhere while a single copy of the loop
+    body is being reduced.) *)
+
+Reserved Notation " t '/' st '===>' t' '/' st' "
+                  (at level 40, st at level 39, t' at level 39).
+
+Inductive cstep : (com * state) -> (com * state) -> Prop :=
+  | CS_AssStep : forall st i a a',
+      a / st ===>a a' ->
+      (i ::= a) / st ===> (i ::= a') / st
+  | CS_Ass : forall st i n,
+      (i ::= (ANum n)) / st ===> SKIP / (t_update st i n)
+  | CS_SeqStep : forall st c1 c1' st' c2,
+      c1 / st ===> c1' / st' ->
+      (c1 ;; c2) / st ===> (c1' ;; c2) / st'
+  | CS_SeqFinish : forall st c2,
+      (SKIP ;; c2) / st ===> c2 / st
+  | CS_IfTrue : forall st c1 c2,
+      IFB BTrue THEN c1 ELSE c2 FI / st ===> c1 / st
+  | CS_IfFalse : forall st c1 c2,
+      IFB BFalse THEN c1 ELSE c2 FI / st ===> c2 / st
+  | CS_IfStep : forall st b b' c1 c2,
+      b / st ===>b b' ->
+          IFB b THEN c1 ELSE c2 FI / st 
+      ===> (IFB b' THEN c1 ELSE c2 FI) / st
+  | CS_While : forall st b c1,
+          (WHILE b DO c1 END) / st
+      ===> (IFB b THEN (c1;; (WHILE b DO c1 END)) ELSE SKIP FI) / st
+
+  where " t '/' st '===>' t' '/' st' " := (cstep (t,st) (t',st')).
+
+(* ################################################################# *)
+(** * Concurrent Imp *)
+
+(** Finally, to show the power of this definitional style, let's
+    enrich Imp with a new form of command that runs two subcommands in
+    parallel and terminates when both have terminated.  To reflect the
+    unpredictability of scheduling, the actions of the subcommands may
+    be interleaved in any order, but they share the same memory and
+    can communicate by reading and writing the same variables. *)
+
+Module CImp.
+
+Inductive com : Type :=
+  | CSkip : com
+  | CAss : id -> aexp -> com
+  | CSeq : com -> com -> com
+  | CIf : bexp -> com -> com -> com
+  | CWhile : bexp -> com -> com
+  (* New: *)
+  | CPar : com -> com -> com.
+
+Notation "'SKIP'" :=
+  CSkip.
+Notation "x '::=' a" :=
+  (CAss x a) (at level 60).
+Notation "c1 ;; c2" :=
+  (CSeq c1 c2) (at level 80, right associativity).
+Notation "'WHILE' b 'DO' c 'END'" :=
+  (CWhile b c) (at level 80, right associativity).
+Notation "'IFB' b 'THEN' c1 'ELSE' c2 'FI'" :=
+  (CIf b c1 c2) (at level 80, right associativity).
+Notation "'PAR' c1 'WITH' c2 'END'" :=
+  (CPar c1 c2) (at level 80, right associativity).
+
+Inductive cstep : (com * state)  -> (com * state) -> Prop :=
+    (* Old part *)
+  | CS_AssStep : forall st i a a',
+      a / st ===>a a' ->
+      (i ::= a) / st ===> (i ::= a') / st
+  | CS_Ass : forall st i n,
+      (i ::= (ANum n)) / st ===> SKIP / (t_update st i n)
+  | CS_SeqStep : forall st c1 c1' st' c2,
+      c1 / st ===> c1' / st' ->
+      (c1 ;; c2) / st ===> (c1' ;; c2) / st'
+  | CS_SeqFinish : forall st c2,
+      (SKIP ;; c2) / st ===> c2 / st
+  | CS_IfTrue : forall st c1 c2,
+      (IFB BTrue THEN c1 ELSE c2 FI) / st ===> c1 / st
+  | CS_IfFalse : forall st c1 c2,
+      (IFB BFalse THEN c1 ELSE c2 FI) / st ===> c2 / st
+  | CS_IfStep : forall st b b' c1 c2,
+      b /st ===>b b' ->
+          (IFB b THEN c1 ELSE c2 FI) / st 
+      ===> (IFB b' THEN c1 ELSE c2 FI) / st
+  | CS_While : forall st b c1,
+          (WHILE b DO c1 END) / st 
+      ===> (IFB b THEN (c1;; (WHILE b DO c1 END)) ELSE SKIP FI) / st
+    (* New part: *)
+  | CS_Par1 : forall st c1 c1' c2 st',
+      c1 / st ===> c1' / st' ->
+      (PAR c1 WITH c2 END) / st ===> (PAR c1' WITH c2 END) / st'
+  | CS_Par2 : forall st c1 c2 c2' st',
+      c2 / st ===> c2' / st' ->
+      (PAR c1 WITH c2 END) / st ===> (PAR c1 WITH c2' END) / st'
+  | CS_ParDone : forall st,
+      (PAR SKIP WITH SKIP END) / st ===> SKIP / st
+  where " t '/' st '===>' t' '/' st' " := (cstep (t,st) (t',st')).
+
+Definition cmultistep := multi cstep.
+
+Notation " t '/' st '===>*' t' '/' st' " :=
+   (multi cstep  (t,st) (t',st'))
+   (at level 40, st at level 39, t' at level 39).
+
+
+(** Among the many interesting properties of this language is the fact
+    that the following program can terminate with the variable [X] set
+    to any value. *)
+
+Definition par_loop : com :=
+  PAR
+    Y ::= ANum 1
+  WITH
+    WHILE BEq (AId Y) (ANum 0) DO
+      X ::= APlus (AId X) (ANum 1)
+    END
+  END.
+
+(** In particular, it can terminate with [X] set to [0]: *)
+
+Example par_loop_example_0:
+  exists st',
+       par_loop / empty_state  ===>* SKIP / st'
+    /\ st' X = 0.
+Proof.
+  eapply ex_intro. split.
+  unfold par_loop.
+  eapply multi_step. apply CS_Par1.
+    apply CS_Ass.
+  eapply multi_step. apply CS_Par2. apply CS_While.
+  eapply multi_step. apply CS_Par2. apply CS_IfStep.
+    apply BS_Eq1. apply AS_Id.
+  eapply multi_step. apply CS_Par2. apply CS_IfStep.
+    apply BS_Eq. simpl.
+  eapply multi_step. apply CS_Par2. apply CS_IfFalse.
+  eapply multi_step. apply CS_ParDone.
+  eapply multi_refl.
+  reflexivity. Qed.
+
+(** It can also terminate with [X] set to [2]: *)
+
+Example par_loop_example_2:
+  exists st',
+       par_loop / empty_state ===>* SKIP / st'
+    /\ st' X = 2.
+Proof.
+  eapply ex_intro. split.
+  eapply multi_step. apply CS_Par2. apply CS_While.
+  eapply multi_step. apply CS_Par2. apply CS_IfStep.
+    apply BS_Eq1. apply AS_Id.
+  eapply multi_step. apply CS_Par2. apply CS_IfStep.
+    apply BS_Eq. simpl.
+  eapply multi_step. apply CS_Par2. apply CS_IfTrue.
+  eapply multi_step. apply CS_Par2. apply CS_SeqStep.
+    apply CS_AssStep. apply AS_Plus1. apply AS_Id.
+  eapply multi_step. apply CS_Par2. apply CS_SeqStep.
+    apply CS_AssStep. apply AS_Plus.
+  eapply multi_step. apply CS_Par2. apply CS_SeqStep.
+    apply CS_Ass.
+  eapply multi_step. apply CS_Par2. apply CS_SeqFinish.
+
+  eapply multi_step. apply CS_Par2. apply CS_While.
+  eapply multi_step. apply CS_Par2. apply CS_IfStep.
+    apply BS_Eq1. apply AS_Id.
+  eapply multi_step. apply CS_Par2. apply CS_IfStep.
+    apply BS_Eq. simpl.
+  eapply multi_step. apply CS_Par2. apply CS_IfTrue.
+  eapply multi_step. apply CS_Par2. apply CS_SeqStep.
+    apply CS_AssStep. apply AS_Plus1. apply AS_Id.
+  eapply multi_step. apply CS_Par2. apply CS_SeqStep.
+    apply CS_AssStep. apply AS_Plus.
+  eapply multi_step. apply CS_Par2. apply CS_SeqStep.
+    apply CS_Ass.
+
+  eapply multi_step. apply CS_Par1. apply CS_Ass.
+  eapply multi_step. apply CS_Par2. apply CS_SeqFinish.
+  eapply multi_step. apply CS_Par2. apply CS_While.
+  eapply multi_step. apply CS_Par2. apply CS_IfStep.
+    apply BS_Eq1. apply AS_Id.
+  eapply multi_step. apply CS_Par2. apply CS_IfStep.
+    apply BS_Eq. simpl.
+  eapply multi_step. apply CS_Par2. apply CS_IfFalse.
+  eapply multi_step. apply CS_ParDone.
+  eapply multi_refl.
+  reflexivity. Qed.
+
+(** More generally... *)
+
+(** **** Exercise: 3 stars, optional (par_body_n__Sn)  *)
+Lemma par_body_n__Sn : forall n st,
+  st X = n /\ st Y = 0 ->
+  par_loop / st ===>* par_loop / (t_update st X (S n)).
+Proof.
+  (* FILL IN HERE *) Admitted.
+(** [] *)
+
+(** **** Exercise: 3 stars, optional (par_body_n)  *)
+Lemma par_body_n : forall n st,
+  st X = 0 /\ st Y = 0 ->
+  exists st',
+    par_loop / st ===>*  par_loop / st' /\ st' X = n /\ st' Y = 0.
+Proof.
+  (* FILL IN HERE *) Admitted.
+(** [] *)
+
+(** ... the above loop can exit with [X] having any value
+    whatsoever. *)
+
+Theorem par_loop_any_X:
+  forall n, exists st',
+    par_loop / empty_state ===>*  SKIP / st'
+    /\ st' X = n.
+Proof.
+  intros n.
+  destruct (par_body_n n empty_state).
+    split; unfold t_update; reflexivity.
+
+  rename x into st.
+  inversion H as [H' [HX HY]]; clear H.
+  exists (t_update st Y 1). split.
+  eapply multi_trans with (par_loop,st). apply H'.
+  eapply multi_step. apply CS_Par1. apply CS_Ass.
+  eapply multi_step. apply CS_Par2. apply CS_While.
+  eapply multi_step. apply CS_Par2. apply CS_IfStep.
+    apply BS_Eq1. apply AS_Id. rewrite t_update_eq.
+  eapply multi_step. apply CS_Par2. apply CS_IfStep.
+    apply BS_Eq. simpl.
+  eapply multi_step. apply CS_Par2. apply CS_IfFalse.
+  eapply multi_step. apply CS_ParDone.
+  apply multi_refl.
+
+  rewrite t_update_neq. assumption. intro X; inversion X.
+Qed.
+
+End CImp.
+
+(* ################################################################# *)
+(** * A Small-Step Stack Machine *)
+
+(** Our last example is a small-step semantics for the stack machine
+    example from the [Imp] chapter. *)
+
+Definition stack := list nat.
+Definition prog  := list sinstr.
+
+Inductive stack_step : state -> prog * stack -> prog * stack -> Prop :=
+  | SS_Push : forall st stk n p',
+    stack_step st (SPush n :: p', stk)      (p', n :: stk)
+  | SS_Load : forall st stk i p',
+    stack_step st (SLoad i :: p', stk)      (p', st i :: stk)
+  | SS_Plus : forall st stk n m p',
+    stack_step st (SPlus :: p', n::m::stk)  (p', (m+n)::stk)
+  | SS_Minus : forall st stk n m p',
+    stack_step st (SMinus :: p', n::m::stk) (p', (m-n)::stk)
+  | SS_Mult : forall st stk n m p',
+    stack_step st (SMult :: p', n::m::stk)  (p', (m*n)::stk).
+
+Theorem stack_step_deterministic : forall st,
+  deterministic (stack_step st).
+Proof.
+  unfold deterministic. intros st x y1 y2 H1 H2.
+  induction H1; inversion H2; reflexivity.
+Qed.
+
+Definition stack_multistep st := multi (stack_step st).
+
+(** **** Exercise: 3 stars, advanced (compiler_is_correct)  *)
+(** Remember the definition of [compile] for [aexp] given in the
+    [Imp] chapter. We want now to prove [compile] correct with respect
+    to the stack machine.
+
+    State what it means for the compiler to be correct according to
+    the stack machine small step semantics and then prove it. *)
+
+Definition compiler_is_correct_statement : Prop 
+  (* REPLACE THIS LINE WITH ":= _your_definition_ ." *). Admitted.
+
+
+Theorem compiler_is_correct : compiler_is_correct_statement.
+Proof.
+(* FILL IN HERE *) Admitted.
+(** [] *)
+
+(** $Date: 2016-12-20 11:28:30 -0500 (Tue, 20 Dec 2016) $ *)
+
+*)
